\documentclass{article}
\input{../../../packagesMemoir}
\input{../../../macros}
\input{../../../amsartMacros}
\lstset{language=matlab}


%opening
\title{Non Linear Programming: Exam 1}
\author{vishvAs vAsuki}

\begin{document}

\maketitle

\section{}
\subsection{Problem setup}
$Pr(x = a_i) = p_i$; $a_1 < a_2 .. < a_n$. P is the probability simplex, formed by all p : $1^{T}p = 1, p \geq 0$.

\subsection{a}
$\ga \leq E[f(x)] = \sum_i p_i f(a_i)\leq \gb$. This is convex: intersection of halfspaces.

\subsection{b}
$Pr(x>\ga) = \sum_{a_i> \ga}p_i \leq \gb$. Convex.

\subsection{c}
$var(X) = E[X^{2}] - (E[X]^{2})\leq \ga$. Not convex.

\subsection{d}
$var(X) = E[X^{2}] - (E[X]^{2})\geq \ga$. Not convex.

\subsection{e}
$quartile(x) = \inf\set{b: Pr(x \leq b) \geq 0.25} \geq \ga \equiv Pr(x < \ga) \leq 0.25$: convex.

\subsection{f}
$quartile(x) \leq \ga$. Convex.

\subsection{g}
$E[f(x)] = \sum p_i f(a_i)$: convex in p.

\subsection{h}
$Pr(\ga \leq x \leq \gb)$: convex in p.

\subsection{i}
var(x) : doesn't look as if it fits any category. \chk

\subsection{j}
quartile(x) : quasilinear.

\section{}
$f^{*}(y) = \sup_{x \in dom(f)} y^{T}x - f(x)$.

\subsection{a}
\begin{eqnarray*}
h_1(x) &=& f(x) + c^{T}x + d\\
h_1^{*}(y) &=& \sup_{x \in dom(f)} y^{T}x - f(x) - c^{T}x - d\\
&=& \sup_{x \in dom(f)} (y - c)^{T}x - f(x) - d\\
&=& f^{*}(y-c) - d \texttt{ if } y\neq c \\
&=&  \sup_{x \in dom(f)} -f(x) - d \texttt{ if } y= c \\
\end{eqnarray*}


\subsection{b}
\begin{eqnarray*}
h_2(x, t) &=& tf(x/t), dom(h_2) = \set{(x, t)|t>0, x/t \in dom(f)}\\
h_2^{*}(y) &=& \sup_{(x, t) \in dom(h_2)} y^{T}x - tf(x/t)\\
&=& \sup_{(x, t) \in dom(h_2)} y^{T}x - tf(x/t)\\
&=& \sup_{(x, t) \in dom(h_2)} t(y^{T}(x/t) - f(x/t))\\
&=& \sup_{t>0}t \sup_{x/t \in dom(f)} (y^{T}(x/t) - f(x/t))\\
&=& \sup_{t>0} t f^{*}(y)\\
\end{eqnarray*}

$dom(h_2^{*}) = \set{y| \exists k: \forall t: tf^{*}(y) \leq k}$.

\subsection{c}
\begin{eqnarray*}
h_3(x) &=& \inf_z \set{f(z)|Az + b = x}\\
h_2^{*}(y) &=& \sup_{x \in dom(h_3)} y^{T}x - \inf_{z: Az + b = x} f(z)\\
&=& \sup_{x = Az + b, z\in dom(f) } y^{T}(Az + b) - \inf_{z} f(z)\\
&=& y^{T}b + \sup_{z\in dom(f) } y^{T}A z - f(z)\\
&=& y^{T}b + f^{*}(A^{T}y)\\
\end{eqnarray*}


\subsection{d}
\begin{eqnarray*}
h_4(x) &=& f(Ax + b)\\
h_4^{*}(y) &=& \sup_{x \in dom(h_4)} y^{T}x - f(Ax + b)\\
\end{eqnarray*}

Consider the optimization problem: $\min_{w, x} f_0(w, x) = f(w) - y^{T}x : Ax + b = w$. The optimal value attained for this problem is $-h_4^{*}(y)$.

Consdier the dual of this problem: $\sup_m -f_0^{*}(A^{T}m - m) - bm$. As strong duality holds, we can say that $-h_4^{*}(y) = \sup_m -f_0^{*}(A^{T}m - m) - bm$.

Now, consider the relationship betweeen $f(y)^{*}$ and $f_0^{*}(y)$.
\begin{eqnarray*}
f^{*}(t) &=& \sup_x t^{T}x - f_0(x) - y^{T}x\\
&=& f_0^{*}(t-y)\\
\therefore -h_4^{*}(y) &=& \sup_m -f^{*}(A^{T}m - m + y) - bm\\
\therefore h_4^{*}(y) &=& \sup_m f^{*}(A^{T}m - m + y) + bm\\
\end{eqnarray*}


\subsection{e}
\begin{assumption}
$dom(f_1) = dom(f_2)$.
\end{assumption}


\begin{eqnarray*}
h_5(x) &=& f_1(x) + f_2(x)\\
h_5^{*}(y) &=& \sup_{x \in dom(f_1) \inters dom(f_2)}y^{T}x - f_1(x) - f_2(x)\\
\texttt{Let }y &=& y_1 + y_2\\
h_5^{*}(y) &=& \sup_{x}y_1^{T}x - f_1(x) + y_2^{T}x - f_2(x)\\
\end{eqnarray*}
\tbc

\subsection{f}
\begin{eqnarray*}
h_6(x) &=& \max \set{f_1(x), f_2(x)}\\
h_6^{*}(y) &=& \sup_{x}y^{T}x - \max \set{f_1(x), f_2(x)}\\
\end{eqnarray*}
\tbc


\section{}
Submitted handwritten.

\section{}
Submitted handwritten.

\section{}
Submitted handwritten.



% \bibliographystyle{plain}
% \bibliography{../linAlg}

\end{document}
